add RBT_set_opt.thy

RBT_height_old.ml
@@ -98,6 +98,8 @@ type compare = LT | GT | EQ;;
 
 type 'a sdlist = Abs_sdlist of 'a list;;
 
+let rec id x = (fun xa -> xa) x;;
+
 let rec plus_nat m n = Nat (Z.add (integer_of_nat m) (integer_of_nat n));;
 
 let one_nat : nat = Nat (Z.of_int 1);;
@@ -248,6 +250,12 @@ let rec insert _A
 
 let rec union _A = foldb _A (insert _A);;
 
+let rec map_filter
+  f x1 = match f, x1 with f, [] -> []
+    | f, x :: xs ->
+        (match f x with None -> map_filter f xs
+          | Some y -> y :: map_filter f xs);;
+
 let rec filtera _A xb xc = Abs_dlist (filter xb (list_of_dlist _A xc));;
 
 let rec balance
@@ -390,16 +398,6 @@ let rec balance
                      Branch (B, vi, vn, vo, vp)),
                s, t, Branch (B, va, vb, vc, vd));;
 
-let rec equal_color x0 x1 = match x0, x1 with R, B -> false
-                      | B, R -> false
-                      | B, B -> true
-                      | R, R -> true;;
-
-let rec bheight
-  = function Empty -> zero_nat
-    | Branch (c, lt, k, v, rt) ->
-        (if equal_color c B then suc (bheight lt) else bheight lt);;
-
 let rec gen_entries
   kvts x1 = match kvts, x1 with
     kvts, Branch (c, l, k, v, r) -> gen_entries (((k, v), r) :: kvts) l
@@ -408,87 +406,9 @@ let rec gen_entries
 
 let rec entries x = gen_entries [] x;;
 
-let rec color_of = function Empty -> B
-                   | Branch (c, uu, uv, uw, ux) -> c;;
-
 let rec skip_red = function Branch (R, l, k, v, r) -> l
                    | Empty -> Empty
                    | Branch (B, va, vb, vc, vd) -> Branch (B, va, vb, vc, vd);;
-
-let rec baliL
-  x0 c t4 = match x0, c, t4 with
-    Branch (R, Branch (R, t1, a, (), t2), b, (), t3), c, t4 ->
-      Branch (R, Branch (B, t1, a, (), t2), b, (), Branch (B, t3, c, (), t4))
-    | Branch (R, Empty, a, (), Branch (R, t2, b, (), t3)), c, t4 ->
-        Branch
-          (R, Branch (B, Empty, a, (), t2), b, (), Branch (B, t3, c, (), t4))
-    | Branch (R, Branch (B, va, vb, vc, vd), a, (), Branch (R, t2, b, (), t3)),
-        c, t4
-        -> Branch
-             (R, Branch (B, Branch (B, va, vb, vc, vd), a, (), t2), b, (),
-               Branch (B, t3, c, (), t4))
-    | Empty, a, t2 -> Branch (B, Empty, a, (), t2)
-    | Branch (B, va, vb, vc, vd), a, t2 ->
-        Branch (B, Branch (B, va, vb, vc, vd), a, (), t2)
-    | Branch (v, Empty, vb, vc, Empty), a, t2 ->
-        Branch (B, Branch (v, Empty, vb, vc, Empty), a, (), t2)
-    | Branch (v, Empty, vb, vc, Branch (B, ve, vf, vg, vh)), a, t2 ->
-        Branch
-          (B, Branch (v, Empty, vb, vc, Branch (B, ve, vf, vg, vh)), a, (), t2)
-    | Branch (v, Branch (B, vf, vg, vh, vi), vb, vc, Empty), a, t2 ->
-        Branch
-          (B, Branch (v, Branch (B, vf, vg, vh, vi), vb, vc, Empty), a, (), t2)
-    | Branch
-        (v, Branch (B, vf, vg, vh, vi), vb, vc, Branch (B, ve, vj, vk, vl)),
-        a, t2
-        -> Branch
-             (B, Branch
-                   (v, Branch (B, vf, vg, vh, vi), vb, vc,
-                     Branch (B, ve, vj, vk, vl)),
-               a, (), t2);;
-
-let rec baliR
-  t1 a x2 = match t1, a, x2 with
-    t1, a, Branch (R, t2, b, (), Branch (R, t3, c, (), t4)) ->
-      Branch (R, Branch (B, t1, a, (), t2), b, (), Branch (B, t3, c, (), t4))
-    | t1, a, Branch (R, Branch (R, t2, b, (), t3), c, (), Empty) ->
-        Branch
-          (R, Branch (B, t1, a, (), t2), b, (), Branch (B, t3, c, (), Empty))
-    | t1, a,
-        Branch (R, Branch (R, t2, b, (), t3), c, (), Branch (B, va, vb, vc, vd))
-        -> Branch
-             (R, Branch (B, t1, a, (), t2), b, (),
-               Branch (B, t3, c, (), Branch (B, va, vb, vc, vd)))
-    | t1, a, Empty -> Branch (B, t1, a, (), Empty)
-    | t1, a, Branch (B, va, vb, vc, vd) ->
-        Branch (B, t1, a, (), Branch (B, va, vb, vc, vd))
-    | t1, a, Branch (v, Empty, vb, vc, Empty) ->
-        Branch (B, t1, a, (), Branch (v, Empty, vb, vc, Empty))
-    | t1, a, Branch (v, Branch (B, ve, vf, vg, vh), vb, vc, Empty) ->
-        Branch
-          (B, t1, a, (), Branch (v, Branch (B, ve, vf, vg, vh), vb, vc, Empty))
-    | t1, a, Branch (v, Empty, vb, vc, Branch (B, vf, vg, vh, vi)) ->
-        Branch
-          (B, t1, a, (), Branch (v, Empty, vb, vc, Branch (B, vf, vg, vh, vi)))
-    | t1, a,
-        Branch
-          (v, Branch (B, ve, vj, vk, vl), vb, vc, Branch (B, vf, vg, vh, vi))
-        -> Branch
-             (B, t1, a, (),
-               Branch
-                 (v, Branch (B, ve, vj, vk, vl), vb, vc,
-                   Branch (B, vf, vg, vh, vi)));;
-
-let rec painta c x1 = match c, x1 with c, Empty -> Empty
-                 | c, Branch (uu, l, a, (), r) -> Branch (c, l, a, (), r);;
-
-let rec skip_black
-  t = (let ta = skip_red t in
-        (match ta with Empty -> ta | Branch (R, _, _, _, _) -> ta
-          | Branch (B, l, _, _, _) -> l));;
-
-let rec filterb _A
-  xb xc = Mapping_RBT (rbtreeify (filter xb (entries (impl_of _A xc))));;
 
 let rec rbt_comp_ins
   c f k v x4 = match c, f, k, v, x4 with
@@ -503,6 +423,97 @@ let rec rbt_comp_ins
           | Gt -> Branch (R, l, x, y, rbt_comp_ins c f k v r));;
 
 let rec rbt_comp_insert_with_key c f k v t = paint B (rbt_comp_ins c f k v t);;
+
+let rec comp_sunion_with
+  c f asa bs = match c, f, asa, bs with
+    c, f, (ka, va) :: asa, (k, v) :: bs ->
+      (match c k ka with Eq -> (ka, f ka va v) :: comp_sunion_with c f asa bs
+        | Lt -> (k, v) :: comp_sunion_with c f ((ka, va) :: asa) bs
+        | Gt -> (ka, va) :: comp_sunion_with c f asa ((k, v) :: bs))
+    | c, f, [], bs -> bs
+    | c, f, asa, [] -> asa;;
+
+let rec skip_black
+  t = (let ta = skip_red t in
+        (match ta with Empty -> ta | Branch (R, _, _, _, _) -> ta
+          | Branch (B, l, _, _, _) -> l));;
+
+let rec compare_height
+  sx s t tx =
+    (match (skip_red sx, (skip_red s, (skip_red t, skip_red tx)))
+      with (Empty, (Empty, (_, Empty))) -> EQ
+      | (Empty, (Empty, (_, Branch (_, _, _, _, _)))) -> LT
+      | (Empty, (Branch (_, _, _, _, _), (Empty, _))) -> EQ
+      | (Empty, (Branch (_, _, _, _, _), (Branch (_, _, _, _, _), Empty))) -> EQ
+      | (Empty,
+          (Branch (_, sa, _, _, _),
+            (Branch (_, ta, _, _, _), Branch (_, txa, _, _, _))))
+        -> compare_height Empty sa ta (skip_black txa)
+      | (Branch (_, _, _, _, _), (Empty, (Empty, Empty))) -> GT
+      | (Branch (_, _, _, _, _), (Empty, (Empty, Branch (_, _, _, _, _)))) -> LT
+      | (Branch (_, _, _, _, _), (Empty, (Branch (_, _, _, _, _), Empty))) -> EQ
+      | (Branch (_, _, _, _, _),
+          (Empty, (Branch (_, _, _, _, _), Branch (_, _, _, _, _))))
+        -> LT
+      | (Branch (_, _, _, _, _), (Branch (_, _, _, _, _), (Empty, _))) -> GT
+      | (Branch (_, sxa, _, _, _),
+          (Branch (_, sa, _, _, _), (Branch (_, ta, _, _, _), Empty)))
+        -> compare_height (skip_black sxa) sa ta Empty
+      | (Branch (_, sxa, _, _, _),
+          (Branch (_, sa, _, _, _),
+            (Branch (_, ta, _, _, _), Branch (_, txa, _, _, _))))
+        -> compare_height (skip_black sxa) sa ta (skip_black txa));;
+
+let rec rbt_comp_union_with_key
+  c f t1 t2 =
+    (match compare_height t1 t1 t2 t2
+      with LT -> folda (rbt_comp_insert_with_key c (fun k v w -> f k w v)) t1 t2
+      | GT -> folda (rbt_comp_insert_with_key c f) t2 t1
+      | EQ -> rbtreeify (comp_sunion_with c f (entries t1) (entries t2)));;
+
+let rec join _A
+  xc xd xe =
+    Mapping_RBT
+      (rbt_comp_union_with_key (the (ccompare _A)) xc (impl_of _A xd)
+        (impl_of _A xe));;
+
+let rec comp_sinter_with
+  c f uv uu = match c, f, uv, uu with
+    c, f, (ka, va) :: asa, (k, v) :: bs ->
+      (match c k ka with Eq -> (ka, f ka va v) :: comp_sinter_with c f asa bs
+        | Lt -> comp_sinter_with c f ((ka, va) :: asa) bs
+        | Gt -> comp_sinter_with c f asa ((k, v) :: bs))
+    | c, f, [], uu -> []
+    | c, f, uv, [] -> [];;
+
+let rec map_option f x1 = match f, x1 with f, None -> None
+                     | f, Some x2 -> Some (f x2);;
+
+let rec rbt_comp_inter_with_key
+  c f t1 t2 =
+    (match compare_height t1 t1 t2 t2
+      with LT ->
+        rbtreeify
+          (map_filter
+            (fun (k, v) ->
+              map_option (fun w -> (k, f k v w)) (rbt_comp_lookup c t2 k))
+            (entries t1))
+      | GT ->
+        rbtreeify
+          (map_filter
+            (fun (k, v) ->
+              map_option (fun w -> (k, f k w v)) (rbt_comp_lookup c t1 k))
+            (entries t2))
+      | EQ -> rbtreeify (comp_sinter_with c f (entries t1) (entries t2)));;
+
+let rec meet _A
+  xc xd xe =
+    Mapping_RBT
+      (rbt_comp_inter_with_key (the (ccompare _A)) xc (impl_of _A xd)
+        (impl_of _A xe));;
+
+let rec filterb _A
+  xb xc = Mapping_RBT (rbtreeify (filter xb (entries (impl_of _A xc))));;
 
 let rec rbt_comp_insert c = rbt_comp_insert_with_key c (fun _ _ nv -> nv);;
 
@@ -521,120 +532,13 @@ let rec inter_list _A
           xc)
         Empty);;
 
-let rec flip_rbt t1 t2 = less_nat (bheight t2) (bheight t1);;
-
-let rec is_empty
-  t = (match t with Empty -> true | Branch (_, _, _, _, _) -> false);;
-
-let rec rbt_joinR
-  l x r =
-    (if less_eq_nat (bheight l) (bheight r) then Branch (R, l, x, (), r)
-      else (match l
-             with Branch (R, la, xa, (), ra) ->
-               Branch (R, la, xa, (), rbt_joinR ra x r)
-             | Branch (B, la, xa, (), ra) -> baliR la xa (rbt_joinR ra x r)));;
-
-let rec rbt_joinL
-  l x r =
-    (if less_eq_nat (bheight r) (bheight l) then Branch (R, l, x, (), r)
-      else (match r
-             with Branch (R, la, xa, (), ra) ->
-               Branch (R, rbt_joinL l x la, xa, (), ra)
-             | Branch (B, la, xa, (), ra) -> baliL (rbt_joinL l x la) xa ra));;
-
-let rec rbt_join
-  l x r =
-    (if less_nat (bheight r) (bheight l) then painta B (rbt_joinR l x r)
-      else (if less_nat (bheight l) (bheight r) then painta B (rbt_joinL l x r)
-             else Branch (B, l, x, (), r)));;
-
-let rec rbt_recolor
-  = function
-    Branch (R, t1, k, v, t2) ->
-      (if equal_color (color_of t1) B && equal_color (color_of t2) B
-        then Branch (B, t1, k, v, t2) else Branch (R, t1, k, v, t2))
-    | Empty -> Empty
-    | Branch (B, va, vb, vc, vd) -> Branch (B, va, vb, vc, vd);;
-
-let rec split_comp
-  comp x1 k = match comp, x1, k with comp, Empty, k -> (Empty, (false, Empty))
-    | comp, Branch (uu, l, a, (), r), x ->
-        (match comp x a with Eq -> (l, (true, r))
-          | Lt -> (let b = split_comp comp l x in
-                   let (l1, ba) = b in
-                   let (bb, l2) = ba in
-                    (l1, (bb, rbt_join l2 a r)))
-          | Gt ->
-            (let b = split_comp comp r x in
-             let (r1, ba) = b in
-             let (bb, r2) = ba in
-              (rbt_join l a r1, (bb, r2))));;
-
-let rec small_rbt t = less_nat (bheight t) (nat_of_integer (Z.of_int 6));;
-
-let rec union_comp
-  comp t1 t2 =
-    (let (t1a, t2a) = (if flip_rbt t1 t2 then (t2, t1) else (t1, t2)) in
-      (if small_rbt t1a then folda (rbt_comp_insert comp) t1a t2a
-        else (match t2a with Empty -> t1a
-               | Branch (_, l2, a, (), r2) ->
-                 (let (l1, (_, r1)) = split_comp comp t1a a in
-                   rbt_join (union_comp comp l1 l2) a
-                     (union_comp comp r1 r2)))));;
-
-let rec rbt_union_rbt_join2 _A
-  xb xc =
-    Mapping_RBT
-      (rbt_recolor
-        (union_comp (the (ccompare _A)) (impl_of _A xb) (impl_of _A xc)));;
-
 let rec uminus_set = function Complement b -> b
                      | Collect_set p -> Collect_set (fun x -> not (p x))
                      | a -> Complement a;;
 
-let rec split_min
-  = function Empty -> failwith "undefined"
-    | Branch (uu, l, a, uv, r) ->
-        (if is_empty l then (a, r)
-          else (let (m, la) = split_min l in (m, rbt_join la a r)));;
-
-let rec rbt_join2
-  l r = (if is_empty r then l else (let a = split_min r in
-                                    let (aa, b) = a in
-                                     rbt_join l aa b));;
-
-let rec inter_comp
-  comp t1 t2 =
-    (let (t1a, t2a) = (if flip_rbt t1 t2 then (t2, t1) else (t1, t2)) in
-      (if small_rbt t1a
-        then rbtreeify
-               (filter
-                 (fun (k, _) ->
-                   equal_option equal_unit (rbt_comp_lookup comp t2a k)
-                     (Some ()))
-                 (entries t1a))
-        else (match t2a with Empty -> Empty
-               | Branch (_, l2, a, (), r2) ->
-                 (let (l1, (ain, r1)) = split_comp comp t1a a in
-                  let l = inter_comp comp l1 l2 in
-                  let r = inter_comp comp r1 r2 in
-                   (if ain then rbt_join l a r else rbt_join2 l r)))));;
-
-let rec rbt_inter_rbt_join2 _A
-  xb xc =
-    Mapping_RBT
-      (rbt_recolor
-        (inter_comp (the (ccompare _A)) (impl_of _A xb) (impl_of _A xc)));;
-
 let rec sup_set (_A1, _A2)
   ba b = match ba, b with
-    RBT_set t1, RBT_set t2 ->
-      (match ccompare _A2
-        with None ->
-          failwith "union RBT_set RBT_set: ccompare = None"
-            (fun _ -> sup_set (_A1, _A2) (RBT_set t1) (RBT_set t2))
-        | Some _ -> RBT_set (rbt_union_rbt_join2 _A2 t1 t2))
-    | ba, Complement b -> Complement (inf_set (_A1, _A2) (uminus_set ba) b)
+    ba, Complement b -> Complement (inf_set (_A1, _A2) (uminus_set ba) b)
     | Complement ba, b -> Complement (inf_set (_A1, _A2) ba (uminus_set b))
     | b, Collect_set a -> Collect_set (fun x -> a x || member (_A1, _A2) x b)
     | Collect_set a, b -> Collect_set (fun x -> a x || member (_A1, _A2) x b)
@@ -693,20 +597,20 @@ let rec sup_set (_A1, _A2)
                   (fun _ -> sup_set (_A1, _A2) (RBT_set rbt) (DList_set dxs))
               | Some _ ->
                 RBT_set (foldb _A1 (fun k -> inserta _A2 k ()) dxs rbt)))
-and inf_set (_A1, _A2)
-  g ga = match g, ga with
-    RBT_set t1, RBT_set t2 ->
-      (match ccompare _A2
-        with None ->
-          failwith "inter RBT_set RBT_set: ccompare = None"
-            (fun _ -> inf_set (_A1, _A2) (RBT_set t1) (RBT_set t2))
-        | Some _ -> RBT_set (rbt_inter_rbt_join2 _A2 t1 t2))
-    | RBT_set rbt1, Set_Monad xs ->
+    | RBT_set rbt1, RBT_set rbt2 ->
         (match ccompare _A2
           with None ->
-            failwith "inter RBT_set Set_Monad: ccompare = None"
-              (fun _ -> inf_set (_A1, _A2) (RBT_set rbt1) (Set_Monad xs))
-          | Some _ -> RBT_set (inter_list _A2 rbt1 xs))
+            failwith "union RBT_set RBT_set: ccompare = None"
+              (fun _ -> sup_set (_A1, _A2) (RBT_set rbt1) (RBT_set rbt2))
+          | Some _ -> RBT_set (join _A2 (fun _ _ -> id) rbt1 rbt2))
+and inf_set (_A1, _A2)
+  g ga = match g, ga with
+    RBT_set rbt1, Set_Monad xs ->
+      (match ccompare _A2
+        with None ->
+          failwith "inter RBT_set Set_Monad: ccompare = None"
+            (fun _ -> inf_set (_A1, _A2) (RBT_set rbt1) (Set_Monad xs))
+        | Some _ -> RBT_set (inter_list _A2 rbt1 xs))
     | RBT_set rbt, DList_set dxs ->
         (match ccompare _A2
           with None ->
@@ -718,6 +622,12 @@ and inf_set (_A1, _A2)
                 failwith "inter RBT_set DList_set: ceq = None"
                   (fun _ -> inf_set (_A1, _A2) (RBT_set rbt) (DList_set dxs))
               | Some _ -> RBT_set (inter_list _A2 rbt (list_of_dlist _A1 dxs))))
+    | RBT_set rbt1, RBT_set rbt2 ->
+        (match ccompare _A2
+          with None ->
+            failwith "inter RBT_set RBT_set: ccompare = None"
+              (fun _ -> inf_set (_A1, _A2) (RBT_set rbt1) (RBT_set rbt2))
+          | Some _ -> RBT_set (meet _A2 (fun _ _ -> id) rbt1 rbt2))
     | DList_set dxs1, Set_Monad xs ->
         (match ceq _A1
           with None ->
@@ -798,32 +708,6 @@ and inf_set (_A1, _A2)
 let rec un_nat_set x y = sup_set (ceq_nat, ccompare_nat) x y;;
 
 let rec int_nat_set x y = inf_set (ceq_nat, ccompare_nat) x y;;
-
-let rec compare_height
-  sx s t tx =
-    (match (skip_red sx, (skip_red s, (skip_red t, skip_red tx)))
-      with (Empty, (Empty, (_, Empty))) -> EQ
-      | (Empty, (Empty, (_, Branch (_, _, _, _, _)))) -> LT
-      | (Empty, (Branch (_, _, _, _, _), (Empty, _))) -> EQ
-      | (Empty, (Branch (_, _, _, _, _), (Branch (_, _, _, _, _), Empty))) -> EQ
-      | (Empty,
-          (Branch (_, sa, _, _, _),
-            (Branch (_, ta, _, _, _), Branch (_, txa, _, _, _))))
-        -> compare_height Empty sa ta (skip_black txa)
-      | (Branch (_, _, _, _, _), (Empty, (Empty, Empty))) -> GT
-      | (Branch (_, _, _, _, _), (Empty, (Empty, Branch (_, _, _, _, _)))) -> LT
-      | (Branch (_, _, _, _, _), (Empty, (Branch (_, _, _, _, _), Empty))) -> EQ
-      | (Branch (_, _, _, _, _),
-          (Empty, (Branch (_, _, _, _, _), Branch (_, _, _, _, _))))
-        -> LT
-      | (Branch (_, _, _, _, _), (Branch (_, _, _, _, _), (Empty, _))) -> GT
-      | (Branch (_, sxa, _, _, _),
-          (Branch (_, sa, _, _, _), (Branch (_, ta, _, _, _), Empty)))
-        -> compare_height (skip_black sxa) sa ta Empty
-      | (Branch (_, sxa, _, _, _),
-          (Branch (_, sa, _, _, _),
-            (Branch (_, ta, _, _, _), Branch (_, txa, _, _, _))))
-        -> compare_height (skip_black sxa) sa ta (skip_black txa));;
 
 let rec compare_height_rbt
   t1 t2 =
