RBT_height.thy
@@ -1,9 +1,79 @@
 theory RBT_height
-  imports "HOL-Library.Code_Target_Nat" "Containers.Containers"
+  imports "HOL-Library.Code_Target_Nat" "Containers.Containers" RBT_set_opt
 begin
+
+(* We define a type of sorted and distinct lists from which we can create an RBT more efficiently
+   than using the built-in function for converting lists into sets. *)
+
+typedef (overloaded) 'a sdlist = "{xs :: ('a :: ccompare) list.
+  case ID CCOMPARE('a) of None \<Rightarrow> xs = [] | Some _ \<Rightarrow> linorder.sorted cless_eq xs \<and> distinct xs}"
+  by (auto intro!: exI[of _ "[]"] split: option.splits)
+     (metis keys_eq_Nil_iff sorted_RBT_Set_keys)
+
+setup_lifting type_definition_sdlist
+
+lemma sset_rbt:
+  fixes xs :: "('a :: ccompare) list"
+    and c :: "'a comparator"
+  assumes assms: "ID ccompare = Some c" "linorder.sorted cless_eq xs" "distinct xs"
+  shows "ord.is_rbt cless (rbtreeify (map (\<lambda>x. (x, ())) xs))"
+  using assms linorder.is_rbt_rbtreeify[OF ID_ccompare[OF assms(1)], of "map (\<lambda>x. (x, ())) xs"]
+  by (auto simp: comp_def)
+
+lift_definition sset :: "('a :: ccompare) sdlist \<Rightarrow> 'a set_rbt" is
+  "\<lambda>xs. rbtreeify (map (\<lambda>x. (x, ())) xs)"
+  using sset_rbt
+  by fastforce
+
+lemma Rep_sdlist_keys:
+  fixes xs :: "('a :: ccompare) sdlist"
+  shows "Rep_sdlist xs = RBT_Set2.keys (sset xs)"
+  by transfer (auto simp: RBT_Impl.keys_def comp_def)
+
+lemma rbt_comp_lookup_iff_in_set:
+  fixes x :: "'a :: ccompare"
+    and xs :: "'a list"
+    and c :: "'a comparator"
+  assumes "ID ccompare = Some c" "linorder.sorted cless_eq xs" "distinct xs"
+  shows "rbt_comp_lookup ccomp (rbtreeify (map (\<lambda>x. (x, ())) xs)) x = Some () \<longleftrightarrow> x \<in> set xs"
+  using linorder.rbt_lookup_rbtreeify[OF ID_ccompare[OF assms(1)], of "map (\<lambda>x. (x, ())) xs"]
+      assms(2,3)
+  by (auto simp: rbt_comp_lookup[OF ID_ccompare'[OF assms(1)]] assms(1) map_of_map_Pair_const
+      comp_def)
+
+lemma RBT_set_sset:
+  fixes xs :: "('a :: ccompare) sdlist"
+  shows "RBT_set (sset xs) = set (Rep_sdlist xs)"
+  unfolding RBT_set_def
+  apply transfer
+  using rbt_comp_lookup_iff_in_set
+  by (fastforce simp: rbtreeify_def split: option.splits)
+
+lemma linorder_sorted_upt: "linorder.sorted (le_of_comp compare) [n..<n']"
+proof -
+  define c :: "nat comparator" where "c = compare"
+  have cl: "class.linorder (le_of_comp c) (lt_of_comp c)"
+    by (auto simp: c_def ID_ccompare ID_Some ccompare_nat_def)
+  show ?thesis
+    using linorder.sorted_sorted_wrt[OF cl] sorted_wrt_mono_rel[OF _ sorted_wrt_upt]
+    by (auto simp: c_def ord_defs(1))
+qed
+
+lift_definition upt_sdlist :: "nat \<Rightarrow> nat \<Rightarrow> nat sdlist" is upt
+  using linorder_sorted_upt
+  by (auto simp: ID_Some ccompare_nat_def split: option.splits)
+
+definition nat_set_upt :: "nat \<Rightarrow> nat \<Rightarrow> nat set" where
+  "nat_set_upt i j = {i..<j}"
+
+lemma nat_set_upt_code[code]: "nat_set_upt i j = RBT_set (sset (upt_sdlist i j))"
+  by (auto simp: nat_set_upt_def RBT_set_sset upt_sdlist.rep_eq)
 
 definition run :: "nat \<Rightarrow> nat \<Rightarrow> nat set" where
   "run i l = {i * l ..< Suc i * l}"
+
+lemma run_code[code]: "run i l = nat_set_upt (i * l) (Suc i * l)"
+  by (auto simp: run_def nat_set_upt_def)
 
 definition compare_height_rbt :: "(nat, unit) mapping_rbt \<Rightarrow> (nat, unit) mapping_rbt \<Rightarrow>
   RBT_Impl.compare" where
@@ -14,7 +84,24 @@ definition compare_height_rbt :: "(nat, unit) mapping_rbt \<Rightarrow> (nat, un
 definition un_nat_set :: "nat set \<Rightarrow> nat set \<Rightarrow> nat set" where
   "un_nat_set X Y = X \<union> Y"
 
-export_code run compare_height_rbt un_nat_set nat_of_integer integer_of_nat RBT_set RBT_Impl.EQ
-  in OCaml module_name RBT_height file_prefix "RBT_height"
+definition int_nat_set :: "nat set \<Rightarrow> nat set \<Rightarrow> nat set" where
+  "int_nat_set X Y = X \<inter> Y"
+
+export_code run compare_height_rbt un_nat_set int_nat_set
+  nat_of_integer integer_of_nat RBT_set RBT_Impl.EQ
+  in OCaml module_name RBT_height file_prefix "RBT_height_old"
+
+declare Set_union_code(1)[code del]
+declare rbt_union_code[code]
+declare Set_inter_code(16)[code del]
+declare rbt_inter_code[code]
+
+(* Set_minus on RBTs not supported in Set_Impl! *)
+declare Set_minus_code[code del]
+declare rbt_minus_code[code]
+
+export_code run compare_height_rbt un_nat_set int_nat_set
+  nat_of_integer integer_of_nat RBT_set RBT_Impl.EQ
+  in OCaml module_name RBT_height file_prefix "RBT_height_opt"
 
 end
