ROOT
@@ -2,6 +2,7 @@ chapter RBT_height
 
 session RBT_height (AFP) = Containers +
   theories
+    RBT_set_opt
     RBT_height
 export_files (in ".") [2]
     "RBT_height.RBT_height:code/**"
